Source/DafnyCore/Verifier/BoogieGenerator.Functions.Wellformedness.cs
@@ -122,10 +122,10 @@ public partial class BoogieGenerator {
       delayer.DoWithDelayedReadsChecks(false, wfo => {
         builder.Add(new CommentCmd("Check well-formedness of preconditions, and then assume them"));
         // If the object has an invariant and f is an instance function, then it can be assumed to check the well-formedness of its preconditions (see well-formedness check for methods for the general principle)
-        /*if (generator.options.Get(CommonOptionBag.CheckInvariants) && f is not Invariant and { IsStatic: false, EnclosingClass: TopLevelDeclWithMembers { Invariant: { } invariant } }) {
+        if (generator.options.Get(CommonOptionBag.CheckInvariants) && f is not Invariant and { IsStatic: false, EnclosingClass: TopLevelDeclWithMembers { Invariant: { } invariant } }) {
           var assertion = invariant.Mention(f.Origin, new ThisExpr(f), generator.program.SystemModuleManager);
           generator.CheckWellformedAndAssume(assertion, wfo, locals, builder, etran, "object invariant as precondition");
-        }*/
+        }
         foreach (AttributedExpression require in ConjunctsOf(f.Req)) {
           if (require.Label != null) {
             require.Label.E = (f is TwoStateFunction ? ordinaryEtran : etran.Old).TrExpr(require.E);
