Source/IntegrationTests/TestFiles/LitTests/LitTest/invariants/ValidIdiom.dfy
@@ -6,13 +6,10 @@ class Nat {
   function Value(): nat
     reads this
   {
-    assert this.invariant(); value // OK, this !in open
+    value // OK, this !in open
   }
-  predicate Valid()
-    reads this
-  {
-    //assert this.invariant(); // NOT OK! function doesn't terminate
-    value >= 0 // OK: this !in open, but does not use this.invariant()
+  invariant Valid(this)
+  static predicate Valid(self: Nat) reads self {
+    self.value >= 0
   }
-  invariant Valid()
 }
