Source/IntegrationTests/TestFiles/LitTests/LitTest/invariants/ValidIdiomError.dfy
@@ -6,13 +6,12 @@ class Nat {
   function Value(): nat
     reads this
   {
-    assert this.invariant(); value // OK, this !in open
+    value
   }
   predicate Valid()
     reads this
   {
-    assert this.invariant(); // NOT OK! function doesn't terminate
-    value >= 0 // OK: this !in open, but does not use this.invariant()
+    assert value >= 0; value >= 0
   }
   invariant Valid()
 }
